Remove explicit key value pairs and replace by explicit equality label matcher

AwesomeDashboards/NodeExporter.lean
@@ -32,8 +32,8 @@ def node_exporter : Exporter := {
   metrics := [node_boot_time_seconds, node_filesystem_avail_bytes, process_cpu_seconds_total, node_network_receive_bytes_total]
 }
 
-def lm : List KeyValuePair := [{key := "__name__", value := "node_filesystem_avail_bytes"}]
-def v := InstantVector.selector {equal := lm} 0
+def lm : List LabelMatcher := [.equal "__name__" "node_filesystem_avail_bytes"]
+def v := InstantVector.selector lm 0
 
 namespace x
 def myPrometheusEnv : Environment := {
@@ -41,15 +41,13 @@ def myPrometheusEnv : Environment := {
 }
 
 #eval InstantVector.typesafe v myPrometheusEnv
-#eval List.map (λ l => l.key) (lm.filter $ is_name)
-#eval List.all (lm.filter $ is_name) (λ l => "node_filesystem_avail_bytes" = l.key )
 
-example : InstantVector.typesafe (InstantVector.selector {equal := lm} 0) myPrometheusEnv := by simp
+example : InstantVector.typesafe (InstantVector.selector lm 0) myPrometheusEnv := by simp
 
 def avail_bytes : InstantVector InstantVectorType.vector := [pql| node_filesystem_avail_bytes-node_filesystem_avail_bytes]
 #eval unitOf myPrometheusEnv avail_bytes
 #eval unitOf myPrometheusEnv [pql| time()]
-#eval RangeVector.unitOf myPrometheusEnv $ RangeVector.selector (LabelMatchers.empty.withName "node_network_receive_bytes_total") 5
+#eval RangeVector.unitOf myPrometheusEnv $ RangeVector.selector [.equal "__name__" "node_network_receive_bytes_total"] 5
 #eval unitOf myPrometheusEnv [pql| rate(node_network_receive_bytes_total{}[5])]
 #eval [pql| rate(node_network_receive_bytes_total{device="vda"}[120])]
 
