Main.lean
@@ -12,9 +12,12 @@ def myPrometheusEnv : Environment := {
 }
 
 def myDashboard : Dashboard myPrometheusEnv := { name := "My Dashboard", panels := [
-    (Panel.graph { promql := { v := [pql| node_filesystem_avail_bytes{fstype="f"} ] } }),
-    (Panel.graph { promql := { v := [pql| process_cpu_seconds_total{job="linux"} ]}}),
-    (Panel.graph { promql := { v := [pql| rate(node_network_receive_bytes_total{device="eth0"}[120]) ]}})
+    (Panel.graph { promql := { v := [pql| node_filesystem_avail_bytes{} ] } }),
+    (Panel.graph { promql := { v := [pql| process_cpu_seconds_total{} ]}}),
+    (Panel.graph { promql := { v := [pql| rate(node_network_receive_bytes_total{device="eth0"}[120]) ]}}),
+    (Panel.table { name := "My tables", columns := [
+      { name := "Free bytes", data := .PrometheusValueColumn [pql| node_filesystem_avail_bytes{} ], index_label := "a" }
+    ] })
 ]}
 
 def main : IO Unit := do
